Assume that the following odd power identity holds
\begin{align}
    \label{eq:odd-power-identity}
    n^{2m+1} = \sum_{r=0}^{m} \sum_{k=1}^{n} \coeffA{m}{r} k^r (n-k)^r
\end{align}
Our main goal is to identify the set of coefficients $\coeffA{m}{0}, \coeffA{m}{1}, \ldots, \coeffA{m}{m}$
such that identity above is true.

Although, the recurrence relation is already given at~\cite{alekseyev2018mathoverflow}, a few key points in proof
are worth to discuss additionally.

The main idea of Alekseyev's approach was to utilize a recurrence relation to evaluate the set of coefficients $\coeffA{m}{r}$
starting from the base case $\coeffA{m}{m}$ and then evaluating the next coefficient $\coeffA{m}{m-1}$
by using backtracking, continuing similarly up to $\coeffA{m}{0}$.

We are going to utilize Binomial theorem $(n-k)^r=\sum_{t=0}^{r} (-1)^t \binom{r}{t} n^{r-t} k^t$ and specific version of Faulhaber's formula
\begin{align*}
    \sum_{k=1}^{n} k^{p}
    = \frac{1}{p+1}\sum_{j=0}^{p} \binom{p+1}{j} \bernoulli{j} n^{p+1-j}
    &= \frac{1}{p+1} \left[ \sum_{j=0}^{p+1} \binom{p+1}{j} \bernoulli{j} n^{p+1-j} \right] - \frac{\bernoulli{p+1}}{p+1} \\
    &= \frac{1}{p+1} \left[ \sum_{j} \binom{p+1}{j} \bernoulli{j} n^{p+1-j} \right] - \frac{\bernoulli{p+1}}{p+1}
\end{align*}
The reason we use modified version of Faulhaber's formula is because its summation bounds can be omitted,
which helps to collapse common terms across complex sums.
Therefore, we expand the sum $\sum_{k=1}^{n} k^{r} (n-k)^{r}$ as follows
\begin{align*}
    &\sum_{k=1}^{n} k^{r} (n-k)^{r}
    = \sum_{t=0}^{r} (-1)^t \binom{r}{t} n^{r-t} \sum_{k=1}^{n} k^{t+r} \\
    &= \sum_{t=0}^{r} (-1)^t \binom{r}{t} n^{r-t} \left[ \left( \frac{1}{t+r+1} \sum_{j} \binom{t+r+1}{j} \bernoulli{j} n^{t+r+1-j} \right) - \frac{\bernoulli{t+r+1}}{t+r+1} \right] \\
    &= \sum_{t=0}^{r} \binom{r}{t} \frac{(-1)^t}{t+r+1} \left[ \sum_{j} \binom{t+r+1}{j} \bernoulli{j} n^{2r+1-j} - \bernoulli{t+r+1} n^{r-t} \right] \\
    &= \left[ \sum_{t=0}^{r} \binom{r}{t} \frac{(-1)^t}{t+r+1} \sum_{j} \binom{t+r+1}{j} \bernoulli{j} n^{2r+1-j}  \right]
    - \left[ \sum_{t=0}^{r} \binom{r}{t} \frac{(-1)^t}{t+r+1} \bernoulli{t+r+1} n^{r-t} \right] \\
    &= \left[ \sum_{j, t} \binom{r}{t} \frac{(-1)^t}{t+r+1} \binom{t+r+1}{j} \bernoulli{j} n^{2r+1-j}  \right]
    - \left[ \sum_{t} \binom{r}{t} \frac{(-1)^t}{t+r+1} \bernoulli{t+r+1} n^{r-t} \right]
\end{align*}
By rearranging the sums we obtain
\begin{equation}
    = \left[ \sum_{j} \bernoulli{j} n^{2r+1-j} \sum_{t} \binom{r}{t} \frac{(-1)^t}{t+r+1} \binom{t+r+1}{j}  \right]
    - \left[ \sum_{t} \binom{r}{t} \frac{(-1)^t}{t+r+1} \bernoulli{t+r+1} n^{r-t} \right]
    \label{eq:rearranging-terms}
\end{equation}
We can notice that
\begin{equation}
    \label{eq:combinatorial-identity}
    \sum_{t} \binom{r}{t} \frac{(-1)^t}{r+t+1} \binom{r+t+1}{j}
    =\begin{cases}
         \frac{1}{(2r+1) \binom{2r}r} & \text{if } j=0\\
         \frac{(-1)^r}{j} \binom{r}{2r-j+1} & \text{if } j>0
    \end{cases}
\end{equation}
An elegant proof of the binomial identity~\eqref{eq:combinatorial-identity} is done by Markus Scheuer in~\cite{scheuer2023mathstackexchange}.

In particular, the equation~\eqref{eq:combinatorial-identity} is zero for $0< t \leq j$.

To utilize the equation~\eqref{eq:combinatorial-identity}, we have to move $j=0$ out of summation
in~\eqref{eq:rearranging-terms} to avoid division by zero in $\frac{(-1)^r}{j}$.
Therefore,
\begin{equation*}
    \begin{split}
        \sum_{k=1}^{n} k^{r} (n-k)^{r}
        &= \frac{1}{(2r+1) \binom{2r}r} n^{2r+1} + \left[ \sum_{j = 1} \bernoulli{j} n^{2r+1-j} \sum_{t} \binom{r}{t} \frac{(-1)^t}{t+r+1} \binom{t+r+1}{j} \right] \\
        &- \left[ \sum_{t=0}^{r} \binom{r}{t} \frac{(-1)^t}{t+r+1} \bernoulli{t+r+1} n^{r-t} \right]
    \end{split}
\end{equation*}
Hence, we simplify the equation above by using~\eqref{eq:combinatorial-identity} so that
\begin{equation*}
    \begin{split}
        \sum_{k=1}^{n} k^{r} (n-k)^{r}
        &= \frac{1}{(2r+1) \binom{2r}r} n^{2r+1}
        + \underbrace{\left[ \sum_{j = 1} \frac{(-1)^r}{j} \binom{r}{2r-j+1} \bernoulli{j} n^{2r-j+1} \right]}_{(\star)} \\
        &- \underbrace{\left[ \sum_{t=0}^{r} \binom{r}{t} \frac{(-1)^t}{t+r+1} \bernoulli{t+r+1} n^{r-t} \right]}_{(\diamond)}
    \end{split}
\end{equation*}
By introducing $\ell=2r-j+1$ to $(\star)$ and $\ell=r-t$ to $(\diamond)$
we collapse the common terms across two sums
\begin{equation*}
    \begin{split}
        \sum_{k=1}^{n} k^{r} (n-k)^{r}
        &= \frac{1}{(2r+1) \binom{2r}r} n^{2r+1}
        + \left[ \sum_{\ell} \frac{(-1)^r}{2r+1-\ell} \binom{r}{\ell} \bernoulli{2r+1-\ell} n^{\ell} \right] \\
        &- \left[ \sum_{\ell} \binom{r}{\ell} \frac{(-1)^{r-\ell}}{2r+1-\ell} \bernoulli{2r+1-\ell} n^{\ell} \right]\\
        &= \frac{1}{(2r+1) \binom{2r}r} n^{2r+1} + 2 \sum_{\mathrm{odd \; \ell}} \frac{(-1)^r}{2r+1-\ell} \binom{r}{\ell} \bernoulli{2r+1-\ell} n^{\ell}
    \end{split}
\end{equation*}
Assuming that $\coeffA{m}{r}$ is defined by the odd-power identity~\eqref{eq:odd-power-identity},
we obtain the following relation for polynomials in $n$
\begin{equation*}
    \sum_{r} \coeffA{m}{r} \frac{1}{(2r+1) \binom{2r}r} n^{2r+1}
    + 2 \sum_{r, \; \mathrm{odd \; \ell}} \coeffA{m}{r} \frac{(-1)^r}{2r+1-\ell} \binom{r}{\ell} \bernoulli{2r+1-\ell} n^{\ell}
    \equiv n^{2m+1}
\end{equation*}
Replacing odd $\ell$ by $\ell = 2k+1$ we get
\begin{align}
    \label{eq:main_relation}
    &\sum_{r} \coeffA{m}{r} \frac{1}{(2r+1) \binom{2r}{r}} n^{2r+1} + 2 \sum_{r, \; k} \coeffA{m}{r} \frac{(-1)^r}{2r-2k} \binom{r}{2k+1} \bernoulli{2r-2k} n^{2k+1}  \equiv n^{2m+1} \\
    &\sum_{r} \coeffA{m}{r} \frac{1}{(2r+1) \binom{2r}{r}} n^{2r+1} + 2 \sum_{r, \; k} \coeffA{m}{r} \frac{(-1)^r}{2r-2k} \binom{r}{2k+1} \bernoulli{2r-2k} n^{2k+1} - n^{2m+1} = 0 \nonumber
\end{align}
We now fix the unused values of $\coeffA{m}{r}$ so that $\coeffA{m}{r} = 0$ for every $r < 0$ or $r > m$.

Taking the coefficient of $n^{2m+1}$ in~\eqref{eq:main_relation} yields
\begin{align}
    \label{eq:question_1}
    \coeffA{m}{m} = (2m+1)\binom{2m}{m}
\end{align}
because $\coeffA{m}{m} \frac{1}{(2m+1) \binom{2m}{m}} = 1$.

That's may not be immediately clear why the coefficient of $n^{2m+1}$ in~\eqref{eq:main_relation} is $(2m+1)\binom{2m}{m}$.
To take the coefficient of $n^{2m+1}$ we fix $r=m$ in $\sum_{r} \coeffA{m}{r} \frac{1}{(2r+1) \binom{2r}{r}} n^{2r+1}$
and $k=m$ in $2 \sum_{r, \; k} \coeffA{m}{r} \frac{(-1)^r}{2r-2k} \binom{r}{2k+1} \bernoulli{2r-2k} n^{2k+1}$, see ~\eqref{eq:main_relation}
\begin{align*}
    &[n^{2m+1}] \left( \sum_{r} \coeffA{m}{r} \frac{1}{(2r+1) \binom{2r}{r}} n^{2r+1}
                    + 2 \sum_{r, \; k} \coeffA{m}{r} \frac{(-1)^r}{2r-2k} \binom{r}{2k+1} \bernoulli{2r-2k} n^{2k+1} - n^{2m+1} \right) \\
    &= \coeffA{m}{m} \frac{1}{(2m+1) \binom{2m}{m}} + 2 \sum_{r} \coeffA{m}{r} \frac{(-1)^r}{2r-2m} \binom{r}{2m+1} \bernoulli{2r-2m} - 1
\end{align*}
We observe that the sum
\begin{align*}
    2 \sum_{r} \coeffA{m}{r} \frac{(-1)^r}{2r - 2m} \binom{r}{2m+1} \bernoulli{2r - 2m}
\end{align*}
does not contribute to the determination of the coefficients because the binomial coefficient
\(\binom{r}{2m+1}\) vanishes for all \(r \leq m\), while \(\coeffA{m}{r} = 0\) for every \(r > m\).
Consequently, all terms in the sum are zero, ensuring no division by zero occurs.


Thus
\begin{align*}
    \coeffA{m}{m} \frac{1}{(2m+1) \binom{2m}{m}}  - 1 = 0
\end{align*}

Taking the coefficient of $n^{2d+1}$ for an integer $d$ in the range $\frac{m}{2} \leq d \leq m-1$ in~\eqref{eq:main_relation} gives
\begin{align*}
    &[n^{2d+1}] \left( \sum_{r=0}^m \coeffA{m}{r} \frac{1}{(2r+1) \binom{2r}{r}} n^{2r+1}
    + 2 \sum_{r=0}^m \sum_k \coeffA{m}{r} \frac{(-1)^r}{2r-2k} \binom{r}{2k+1} \bernoulli{2r-2k} n^{2k+1} - n^{2m+1} \right) \\
    &= \coeffA{m}{d} \frac{1}{(2d+1) \binom{2d}{d}} + 2 \sum_{r=0}^m \coeffA{m}{r} \frac{(-1)^r}{2r-2d} \binom{r}{2d+1} \bernoulli{2r-2d}.
\end{align*}

For every $d \geq \frac{m}{2}$, the binomial coefficient $\binom{r}{2d+1} = 0$ for all $r \leq m$, since $2d+1 > m$.

As a particular example, when $r = m$ and $d = \frac{m}{2}$, we have
\begin{align*}
    \binom{m}{m+1} = 0.
\end{align*}

Therefore, the entire sum involving $\binom{r}{2d+1}$ vanishes, and we conclude
\begin{align*}
    \coeffA{m}{d} \frac{1}{(2d+1) \binom{2d}{d}} = 0 \implies \coeffA{m}{d} = 0.
\end{align*}

Hence, for all integers $d$ such that $\frac{m}{2} \leq d \leq m-1$, the coefficient $\coeffA{m}{d} = 0$.

In contrast, for values $d \leq \frac{m}{2} - 1$, the binomial coefficient $\binom{r}{2d+1}$ can be nonzero; for instance, if $r = m$ and $d = \frac{m}{2} - 1$, then
\begin{align*}
    \binom{m}{m - 1} \neq 0,
\end{align*}
allowing the corresponding terms to contribute to the determination of $\coeffA{m}{d}$.

Taking the coefficient of $n^{2d+1}$ for $d$ in the range $\frac{m}{4} \leq d < \frac{m}{2}$ in~\eqref{eq:main_relation}, we obtain
\begin{align}
    \label{eq:question_3}
    \coeffA{m}{d} \frac{1}{(2d+1) \binom{2d}{d}}
    + 2 (2m+1) \binom{2m}{m} \binom{m}{2d+1} \frac{(-1)^m}{2m - 2d} \bernoulli{2m - 2d} = 0.
\end{align}

Solving for $\coeffA{m}{d}$ yields
\begin{equation*}
    \coeffA{m}{d}
    = (-1)^{m-1} \frac{(2m+1)!}{d! \, d! \, m! \, (m - 2d - 1)!} \cdot \frac{1}{m - d} \bernoulli{2m - 2d}.
\end{equation*}

Proceeding recursively, we can compute each coefficient $\coeffA{m}{r}$ for integers $r$ in the ranges
\[
    \frac{m}{2^{s+1}} \leq r < \frac{m}{2^s}, \quad \text{for } s = 1, 2, \ldots
\]
by using previously computed values $\coeffA{m}{d}$ for $d > r$, via the relation:
\begin{equation*}
    \coeffA{m}{r} =
    (2r+1) \binom{2r}{r} \sum_{d = 2r+1}^{m}
    \coeffA{m}{d} \binom{d}{2r+1} \frac{(-1)^{d-1}}{d - r} \bernoulli{2d - 2r}.
\end{equation*}


Finally, we are capable to define the following recurrence relation for coefficient $\coeffA{m}{r}$
\begin{definition} (Definition of coefficient $\coeffA{m}{r}$.)
    \begin{equation}
        \label{eq:definition_coefficient_a}
        \coeffA{m}{r} =
        \begin{cases}
        (2r+1)
            \binom{2r}{r} & \mathrm{if} \; r=m \\
            (2r+1) \binom{2r}{r} \sum_{d \geq 2r+1}^{m} \coeffA{m}{d} \binom{d}{2r+1} \frac{(-1)^{d-1}}{d-r}
            \bernoulli{2d-2r} & \mathrm{if} \; 0 \leq r<m \\
            0 & \mathrm{if} \; r<0 \; \mathrm{or} \; r>m
        \end{cases}
    \end{equation}
\end{definition}
where $\bernoulli{t}$ are Bernoulli numbers~\cite{bateman1953higher}.
It is assumed that $\bernoulli{1}=\frac{1}{2}$.

For example,
\input{sections/figures/05_fig_coefficients_a}

Properties of the coefficients $\coeffA{m}{r}$
\begin{itemize}
    \item $\coeffA{m}{m} = \binom{2m}{m}$
    \item $\coeffA{m}{r} = 0$ for $m < 0$ and $r > m$
    \item $\coeffA{m}{r} = 0$ for $r < 0$
    \item $\coeffA{m}{r} = 0$ for $\frac{m}{2} \leq r < m$
    \item $\coeffA{m}{0} = 1$ for $m \geq 0$
    \item $\coeffA{m}{r}$ are integers for $m \leq 11$
    \item Row sums: $\sum_{r=0}^{m} \coeffA{m}{r} = 2^{2m+1} - 1$
\end{itemize}
