\begin{question}
    Although, a proof of combinatorial identity~\eqref{eq:combinatorial-identity} is already present, it is good
    to point out literature or more context on it.
    Reference to a book or article with deeper discussion.
\end{question}
\begin{question}
    I have struggle to understand the equation~\eqref{eq:question_1}, it takes the coefficient of $n^{2m+1}$ meaning that
    we substitute $r=m$ into~\eqref{eq:main_relation} evaluating it, if I understand it properly.
    So that coefficient of $n^{2m+1}$ is
    \begin{align*}
         \coeffA{m}{m} \frac{1}{(2m+1) \binom{2m}m} n^{2m+1}
        + 2 \sum_{k} \coeffA{m}{m} \frac{(-1)^m}{2m-2k} \binom{m}{2k+1} \bernoulli{2m-2k} n^{2k+1} = 1
    \end{align*}
    It implies that coefficient of $n^{2m+1}$ in following sum is zero
    \begin{align*}
        2 \sum_{k} \coeffA{m}{m} \frac{(-1)^m}{2m-2k} \binom{m}{2k+1} \bernoulli{2m-2k} n^{2k+1} = 0
    \end{align*}
    So that
    \begin{align*}
        \coeffA{m}{m} \frac{1}{(2m+1) \binom{2m}m} = 1; \quad \quad \coeffA{m}{m} = (2m+1)\binom{2m}{m}
    \end{align*}
    Which is indeed true because $\binom{m}{2k+1} = 0$ as $k=m$.
\end{question}
\begin{question}
    Almost the same problem with equation~\eqref{eq:question_2},
    taking the coefficient of $n^{2d+1}$ for an integer $d$ in the range $\frac{m}{2} \leq d < m$, we get
    \begin{align*}
        \coeffA{m}{d} = 0
    \end{align*}
    Let be $r=d$ in~\eqref{eq:main_relation}
    \begin{align*}
        \coeffA{m}{d} \frac{1}{(2d+1) \binom{2d}d} n^{2d+1}
        + 2 \sum_{k} \coeffA{m}{d} \frac{(-1)^d}{2d-2k} \binom{d}{2k+1} \bernoulli{2d-2k} n^{2k+1} = 0
    \end{align*}
    Let be $d=m-1$ then again same principle
    \begin{align*}
        2 \sum_{k} \coeffA{m}{d} \frac{(-1)^d}{2d-2k} \binom{d}{2k+1} \bernoulli{2d-2k} n^{2k+1} = 0
    \end{align*}
    because $\binom{m-1}{2k+1}=0$ as $k=m-1$.
\end{question}
To summarize, the value of $k$ should be in range $k \leq \frac{d-1}{2}$ so that binomial coefficient $\binom{d}{2k+1}$
is non-zero.
